CircuitSATEncoding.dfy
@@ -1,5 +1,132 @@
-type Gates=set<string>
-type Variable=string
-type VariableSet=set<Variable>
+include "turing_machine.dfy"
+datatype gate = AND (i1:nat,i2:nat)| OR(i1:nat,i2:nat) | NOT(i:nat) | VARIABLE(x:string) 
+type circuit=seq<gate>
+type certificate=seq<string>
+function natToString(n: nat): string {
+    match n
+    case 0 => "0" case 1 => "1" case 2 => "2" case 3 => "3" case 4 => "4"
+    case 5 => "5" case 6 => "6" case 7 => "7" case 8 => "8" case 9 => "9"
+    case _ => natToString(n / 10) + natToString(n % 10)
+  }
+function stringToNat(s:string): Option<nat> {
+    if |s|!=0 then
+        stringToNat'(s,0)
+    else
+        None
+}
+function stringToNat'(s:string,pos:nat):Option<nat>
+    requires pos<=|s|
+    decreases |s|-pos
+{
+    if pos==|s| then
+         Some(0)
+    else
+        if s[pos] >='0' && s[pos]<='9' then
+            match stringToNat'(s,pos+1)
+                case Some(n) => Some(n*10+(s[pos] as int - '0' as int))    
+                case None => None
+        else
+            None
+}
 
+predicate isCircuitValid (c:circuit)
+{
+     forall pos:nat :: 0<=pos<|c| ==>  match c[pos]
+        case AND (i1,i2) => i1>=0 && i1>=0 && i1<pos && i2<pos
+        case OR (i1,i2) => i1>=0 && i1>=0 && i1<pos && i2<pos
+        case NOT (i) => i>=0 && i<pos
+        case VARIABLE (_) => true 
+}
 
+function gateToString (g:gate) : string
+{
+    match g
+        case AND (i1,i2) => "AND: "+natToString(i1)+" "+natToString(i2)    
+        case OR (i1,i2) => "OR: "+natToString(i1)+" "+natToString(i2)
+        case NOT (i) => "Not: "+natToString(i)
+        case VARIABLE (x) => x
+}
+function circuitToInput (c:circuit) : seq<string>
+{
+    circuitToInput'(c,0)
+}
+function circuitToInput' (c:circuit,pos:nat) :seq<string>
+    requires |c|>=pos
+    decreases |c|-pos
+{
+    if pos==|c| then []
+    else [gateToString(c[pos])] + circuitToInput'(c,pos+1)
+}
+function inputToCircuit (input:seq<string>) : circuit
+{
+    input
+}
+predicate isCertificateValid (c:circuit,k:certificate)
+{
+    forall pos:nat:: pos<|c| ==> (
+            match c[pos] 
+                case VARIABLE(x) => exists poz:nat :: poz<|k| && (
+                    k[poz]==x+" : "+"1" || k[poz]==x+" : "+"0") 
+                case _ => true
+        )
+}
+function getValueFromCertificate (v:string,k:certificate):Option<bool>
+    ensures getValueFromCertificate(v,k)!=None <==>exists poz:nat :: poz<|k| && (
+                    k[poz]==v+" : "+"1" || k[poz]==v+" : "+"0")
+
+{
+    getValueFromCertificate'(v,k,0)
+}
+function getValueFromCertificate'(v:string,k:certificate,pos:nat):Option<bool>
+    requires pos<=|k|
+    decreases |k|-pos
+    ensures getValueFromCertificate'(v,k,pos)!=None <==>exists poz:nat :: poz<|k| && (
+                    k[poz]==v+" : "+"1" || k[poz]==v+" : "+"0")
+    requires forall poz:nat ::poz<pos ==> ( k[poz]!=v+" : "+"1" && k[poz]!=v+" : "+"0")
+    ensures forall poz:nat ::poz<pos ==> ( k[poz]!=v+" : "+"1" && k[poz]!=v+" : "+"0")
+{
+    if pos==|k| then None
+    else
+        if k[pos]==v+" : "+"1" then 
+            Some(true)
+        else
+            if  k[pos]==v+" : "+"0" then
+            Some(false)
+        else 
+            getValueFromCertificate'(v,k,pos+1)
+}
+predicate solveCircuit(c:circuit,k:certificate)
+    requires isCircuitValid(c)
+    requires isCertificateValid(c,k)
+    requires |c|>=1
+{
+    solveCircuit'(c,k,|c|-1)
+}
+predicate solveCircuit'(c:circuit,k:certificate,pos:nat)
+    requires isCircuitValid(c)
+    requires isCertificateValid(c,k)
+    requires |c|>=1
+    requires pos<|c|
+    decreases pos
+{
+
+    match c[pos]
+        case AND (i1,i2) =>     solveCircuit'(c,k,i1) && solveCircuit'(c,k,i2)
+        case OR (i1,i2) =>      solveCircuit'(c,k,i1) || solveCircuit'(c,k,i2)
+        case NOT (i) =>         solveCircuit'(c,k,i)
+        case VARIABLE (x) =>     match getValueFromCertificate(x,k)
+                                        case Some(st) => st
+}
+ghost function generateCKTSATLanguage ():Language 
+{
+    generateCKTSATLanguage'({})
+}
+predicate checkSatisfaction(c:circuit)
+    requires isCircuitValid(c)
+{
+    exists k:certificate :: isCertificateValid(c,k) && solveCircuit(c,k)
+}
+ghost predicate isThatActuallyTheCKTSATLanguage (l:Language) 
+{
+    forall input:seq<string> :: (input in l) ==> 
+}
